LeanSAT/Reflect/BVExpr/BitBlast/Lemmas/ShiftRight.lean
@@ -1,0 +1,150 @@
+import LeanSAT.Reflect.BVExpr.BitBlast.Lemmas.Basic
+import LeanSAT.Reflect.BVExpr.BitBlast.Impl.ShiftRight
+
+open AIG
+
+namespace BVExpr
+namespace bitblast
+namespace blastShiftRightConst
+
+theorem go_getRef_aux (aig : AIG BVBit) (distance : Nat) (input : AIG.RefStream aig w)
+    (curr : Nat) (hcurr : curr ≤ w) (s : AIG.RefStream aig curr)
+    : ∀ (idx : Nat) (hidx : idx < curr) (hfoo),
+        (go aig input distance curr hcurr s).stream.getRef idx (by omega)
+          =
+        (s.getRef idx hidx).cast hfoo := by
+  intro idx hidx
+  generalize hgo : go aig input distance curr hcurr s = res
+  unfold go at hgo
+  split at hgo
+  . dsimp at hgo
+    split at hgo
+    . rw [← hgo]
+      intros
+      rw [go_getRef_aux]
+      rw [AIG.RefStream.getRef_push_ref_lt]
+    . rw [← hgo]
+      intros
+      rw [go_getRef_aux]
+      rw [AIG.RefStream.getRef_push_ref_lt]
+      . simp only [Ref.cast, Ref.mk.injEq]
+        rw [AIG.RefStream.getRef_cast]
+        . simp
+        . assumption
+      . apply go_le_size
+  . dsimp at hgo
+    rw [← hgo]
+    simp only [Nat.le_refl, RefStream.getRef, Ref_cast', Ref.mk.injEq, true_implies]
+    congr
+    . omega
+    . simp
+termination_by w - curr
+
+theorem go_getRef (aig : AIG BVBit) (distance : Nat) (input : AIG.RefStream aig w)
+    (curr : Nat) (hcurr : curr ≤ w) (s : AIG.RefStream aig curr)
+    : ∀ (idx : Nat) (hidx : idx < curr),
+        (go aig input distance curr hcurr s).stream.getRef idx (by omega)
+          =
+        (s.getRef idx hidx).cast (by apply go_le_size) := by
+  intros
+  apply go_getRef_aux
+
+theorem go_denote_mem_prefix (aig : AIG BVBit) (distance : Nat) (input : AIG.RefStream aig w)
+    (curr : Nat) (hcurr : curr ≤ w) (s : AIG.RefStream aig curr) (start : Nat) (hstart)
+  : ⟦
+      (go aig input distance curr hcurr s).aig,
+      ⟨start, by apply Nat.lt_of_lt_of_le; exact hstart; apply go_le_size⟩,
+      assign
+    ⟧
+      =
+    ⟦aig, ⟨start, hstart⟩, assign⟧ := by
+  apply denote.eq_of_aig_eq (entry := ⟨aig, start,hstart⟩)
+  apply IsPrefix.of
+  . intros
+    apply go_decl_eq
+  . intros
+    apply go_le_size
+
+theorem go_eq_eval_getLsb (aig : AIG BVBit) (distance : Nat) (input : AIG.RefStream aig w)
+    (assign : Assignment) (curr : Nat) (hcurr : curr ≤ w) (s : AIG.RefStream aig curr)
+    : ∀ (idx : Nat) (hidx1 : idx < w) (hidx2 : curr ≤ idx),
+        ⟦
+          (go aig input distance curr hcurr s).aig,
+          (go aig input distance curr hcurr s).stream.getRef idx hidx1,
+          assign.toAIGAssignment
+        ⟧
+          =
+        if hidx:(distance + idx) < w then
+          ⟦aig, input.getRef (distance + idx) (by omega), assign.toAIGAssignment⟧
+        else
+          false
+        := by
+  intro idx hidx1 hidx2
+  generalize hgo : go aig input distance curr hcurr s = res
+  unfold go at hgo
+  split at hgo
+  . dsimp at hgo
+    cases Nat.eq_or_lt_of_le hidx2 with
+    | inl heq =>
+      split at hgo
+      . split
+        . rw [← hgo]
+          rw [go_getRef]
+          rw [AIG.RefStream.getRef_push_ref_eq']
+          . rw [go_denote_mem_prefix]
+            . simp [heq]
+            . simp [Ref.hgate]
+          . rw [heq]
+        . omega
+      . split
+        . omega
+        . rw [← hgo]
+          rw [go_getRef]
+          rw [AIG.RefStream.getRef_push_ref_eq']
+          . rw [go_denote_mem_prefix]
+            . simp
+            . simp [Ref.hgate]
+          . rw [heq]
+    | inr =>
+      split at hgo
+      . split
+        all_goals
+          next hidx =>
+            rw [← hgo]
+            rw [go_eq_eval_getLsb]
+            . simp [hidx]
+            . omega
+      . split
+        . omega
+        . next hidx =>
+          rw [← hgo]
+          rw [go_eq_eval_getLsb]
+          . simp [hidx]
+          . omega
+  . omega
+termination_by w - curr
+
+end blastShiftRightConst
+
+@[simp]
+theorem blastShiftRight_eq_eval_getLsb (aig : AIG BVBit) (target : ShiftTarget aig w)
+    (assign : Assignment)
+    : ∀ (idx : Nat) (hidx : idx < w),
+        ⟦
+          (blastShiftRightConst aig target).aig,
+          (blastShiftRightConst aig target).stream.getRef idx hidx,
+          assign.toAIGAssignment
+        ⟧
+          =
+        if hidx:(target.distance + idx) < w then
+          ⟦aig, target.stream.getRef (target.distance + idx) (by omega), assign.toAIGAssignment ⟧
+        else
+          false
+        := by
+  intros
+  unfold blastShiftRightConst
+  apply blastShiftRightConst.go_eq_eval_getLsb
+  omega
+
+end bitblast
+end BVExpr
